Fully proved soundness for programs with line numbers

src/TraceLogic2020WithLines.v
@@ -29,8 +29,8 @@ Fixpoint subprogram_line_diff (c : com) :=
   | CAsgn _ _ _ => 1
   | CArrAsgn _ _ _ _ => 1
   | CSeq _ c1 c2 => subprogram_line_diff c1 + subprogram_line_diff c2
-  | CIf _ _ c1 c2 => 1 + subprogram_line_diff c1 + subprogram_line_diff c2
-  | CWhile _ _ c => 1 + subprogram_line_diff c
+  | CIf _ _ c1 c2 => 1 + subprogram_line_diff c1 + 1 + subprogram_line_diff c2 + 1
+  | CWhile _ _ c => 1 + 1 + subprogram_line_diff c + 1
   end.
 
 Inductive HasConsistentLineNumbers : nat -> com -> Prop :=
@@ -45,17 +45,13 @@ Inductive HasConsistentLineNumbers : nat -> com -> Prop :=
       HasConsistentLineNumbers (line + subprogram_line_diff c1) c2 ->
       HasConsistentLineNumbers line (CSeq line c1 c2)
   | HasConsistentLineNumbersIf (line : nat) (b : bexp) (c1 c2 : com) :
-      HasConsistentLineNumbers (S line) c1 ->
-      HasConsistentLineNumbers ((S line) + subprogram_line_diff c1) c2 ->
+      HasConsistentLineNumbers (line + 1) c1 ->
+      HasConsistentLineNumbers (line + 1 + subprogram_line_diff c1 + 1) c2 ->
       HasConsistentLineNumbers line (CIf line b c1 c2)
   | HasConsistentLineNumbersWhile (line : nat) (b : bexp) (c : com) :
-      HasConsistentLineNumbers (S (S line)) c ->
+      HasConsistentLineNumbers (line + 1 + 1) c ->
       HasConsistentLineNumbers line (CWhile line b c)
   .
-
-Ltac assert_compute H E :=
-  let v := eval compute in E in
-  assert (H : E = v) by reflexivity.
 
 Example consistent_line_numbers_example :
   HasConsistentLineNumbers 0 (
@@ -63,7 +59,7 @@ Example consistent_line_numbers_example :
       CIf 2 BTrue (
         CAsgn 3 "x" (ANum 3)
       ) (
-        CSkip 4
+        CSkip 5
       )
     )
   ).
@@ -92,7 +88,7 @@ Example immediate_subprogram_example :
     CIf 2 BTrue (
       p2
     ) (
-      CSkip 4
+      CSkip 5
     )
   ) in
   IsImmediateSubprogram p1 p2.
@@ -102,6 +98,7 @@ Qed.
 
 (* reflexive transitive closure *)
 Definition IsSubprogram := clos_refl_trans com IsImmediateSubprogram.
+Hint Unfold IsSubprogram : core.
 
 Example subprogram_example :
   let p2 := (
@@ -110,9 +107,9 @@ Example subprogram_example :
   let p1 := (
     CWhile 0 BTrue (
       CIf 2 BTrue (
-        CAsgn 3 "x" (ANum 3)
+        p2
       ) (
-        CSkip 4
+        CSkip 5
       )
     )
   ) in
@@ -129,6 +126,25 @@ Qed.
 Inductive Timepoint : Type :=
   | TimepointAt (line : nat) (enclIts : list nat)
   .
+
+(* denoted as ${start}_p$ in the paper *)
+Definition line_before (subprogram : com) :=
+  match subprogram with
+    | CSkip line => line
+    | CAsgn line _ _ => line
+    | CArrAsgn line _ _ _ => line
+    | CSeq line _ _ => line
+    | CIf line _ _ _ => line
+    | CWhile line _ _ => line
+  end.
+Definition time_before (subprogram : com) (enclIts : list nat) :=
+  TimepointAt (line_before subprogram) enclIts.
+
+(* denoted as ${end}_p$ in the paper *)
+Definition line_after (subprogram : com) :=
+  line_before subprogram + subprogram_line_diff subprogram.
+Definition time_after (subprogram : com) (enclIts : list nat) :=
+  TimepointAt (line_after subprogram) enclIts.
 
 (* denoted as $v \in S_V$ in the paper *)
 Definition IntVar : Type := Timepoint -> Z.
@@ -151,14 +167,940 @@ Parameter beval : forall (tp : Timepoint), bexp -> bool.
 
 (* we'll need to know the last loop iteration of each line, denoted as $n_s \in S_n$ in the paper. also denoted ${lastIt}_s$ *)
 Parameter LastLoopIteration : forall (t : Timepoint), nat.
-Axiom last_loop_iteration_cond_is_false : forall line cond c enclIts,
-  IsSubprogram program (CWhile line cond c) ->
-  let it := LastLoopIteration (TimepointAt line enclIts) in
-  beval (TimepointAt line (it :: enclIts)) cond = false.
-Axiom last_loop_iteration_before_cond_is_true : forall line cond c it enclIts,
-  IsSubprogram program (CWhile line cond c) ->
-  it < LastLoopIteration (TimepointAt line enclIts) ->
-  beval (TimepointAt (S line) (it :: enclIts)) cond = true.
+Axiom last_loop_iteration_cond_is_false : forall line cond c,
+  let subprogram := CWhile line cond c in
+  IsSubprogram program subprogram ->
+  forall enclIts,
+  let it := LastLoopIteration (time_before subprogram enclIts) in
+  beval (TimepointAt (line_before subprogram + 1) (it :: enclIts)) cond = false.
+Axiom last_loop_iteration_before_cond_is_true : forall line cond c,
+  let subprogram := CWhile line cond c in
+  IsSubprogram program subprogram ->
+  forall it enclIts,
+  it < LastLoopIteration (time_before subprogram enclIts) ->
+  beval (TimepointAt (line_before subprogram + 1) (it :: enclIts)) cond = true.
 
 (* NOTE: since it's easier to add/remove elements from the heed of lists,
 enclosing iterations (enclIts) are saved in reverse order, like a stack *)
+
+
+(* ================================================================= *)
+(* Trace Logic semantics                                             *)
+(* ================================================================= *)
+
+(* equality between timepoints *)
+Definition EqInt (v : IntVar) (tp1 tp2 : Timepoint) : Prop :=
+  v tp1 = v tp2.
+Definition EqArray (v : ArrayVar) (tp1 tp2 : Timepoint) : Prop :=
+  forall (pos : Z), v pos tp1 = v pos tp2.
+Definition EqAll (tp1 tp2 : Timepoint) : Prop :=
+  List.Forall (fun v => EqInt v tp1 tp2) AllIntVars
+  /\ List.Forall (fun v => EqArray v tp1 tp2) AllArrayVars.
+
+(* timepoints differing by a single assignment *)
+Definition Update (v : IntVar) (e : aexp) (tp1 tp2 : Timepoint) : Prop :=
+  v tp2 = aeval tp1 e
+  /\ List.Forall (fun v' => v' = v \/ EqInt v' tp1 tp2) AllIntVars
+  /\ List.Forall (fun v' => EqArray v' tp1 tp2) AllArrayVars.
+Definition UpdateArray (v : ArrayVar) (e1 e2 : aexp) (tp1 tp2 : Timepoint) : Prop :=
+  (forall (pos : Z), pos = aeval tp1 e1 \/ v pos tp2 = v pos tp1)
+  /\ v (aeval tp1 e1) tp2 = aeval tp1 e2
+  /\ List.Forall (fun v' => EqInt v' tp1 tp2) AllIntVars
+  /\ List.Forall (fun v' => v' = v \/ EqArray v' tp1 tp2) AllArrayVars.
+
+
+(* define the Trace Logic semantics of a subprogram, denoted by double square brackets in the paper *)
+(* unlike the paper, this does not use `Reach` but rather recursion *)
+(* also unlike the paper, since we have unique timepoints we need to sprinkle some more $EqAll$ *)
+Fixpoint trace_logic_semantics (enclIts : list nat) (subprogram : com) : Prop :=
+  match subprogram with
+    | CSkip line =>
+        EqAll (time_before subprogram enclIts) (time_after subprogram enclIts)
+    | CAsgn line v e =>
+        Update (IntVarByName v) e (time_before subprogram enclIts) (time_after subprogram enclIts)
+    | CArrAsgn line v e1 e2 =>
+        UpdateArray (ArrayVarByName v) e1 e2 (time_before subprogram enclIts) (time_after subprogram enclIts)
+    | CSeq line c1 c2 =>
+        trace_logic_semantics enclIts c1
+        /\ trace_logic_semantics enclIts c2
+    | CIf line cond c1 c2 =>
+        let c := if beval (time_before subprogram enclIts) cond then c1 else c2 in
+        EqAll (time_before subprogram enclIts) (time_before c enclIts)
+        /\ EqAll (time_after c enclIts) (time_after subprogram enclIts)
+        /\ trace_logic_semantics enclIts c
+    | CWhile line cond c =>
+        let lastIt := LastLoopIteration (time_before subprogram enclIts) in
+        let time_before_condition := TimepointAt (line_before subprogram + 1) in
+        EqAll (time_before subprogram enclIts) (time_before_condition (0 :: enclIts))
+        /\ (forall (it : nat), it < lastIt ->
+          beval (time_before_condition (it :: enclIts)) cond = true
+          /\ EqAll (time_before_condition (it :: enclIts)) (time_before c (it :: enclIts))
+          /\ EqAll (time_after c (it :: enclIts)) (time_before_condition (S it :: enclIts))
+          /\ trace_logic_semantics (it :: enclIts) c
+        )
+        /\ beval (time_before_condition (lastIt :: enclIts)) cond = false
+        /\ EqAll (time_before_condition (lastIt :: enclIts)) (time_after subprogram enclIts)
+  end.
+
+Definition trace_logic_semantics_for_program := trace_logic_semantics (@nil nat) program.
+
+
+(* ================================================================= *)
+(* Trace Logic small-step semantics                                  *)
+(* ================================================================= *)
+
+(* SOS stands for small-step operational semantics *)
+(* from Appendix A *)
+Inductive ReachSOS : Timepoint -> Prop :=
+  | ReachSOSStart :
+      ReachSOS (time_before program (@nil nat))
+  | ReachSOSSkip enclIts line :
+      let subprogram := CSkip line in
+      IsSubprogram program subprogram ->
+      ReachSOS (time_before subprogram enclIts) ->
+      ReachSOS (time_after subprogram enclIts)
+  | ReachSOSAsgn enclIts line v e :
+      let subprogram := CAsgn line v e in
+      IsSubprogram program subprogram ->
+      ReachSOS (time_before subprogram enclIts) ->
+      ReachSOS (time_after subprogram enclIts)
+  | ReachSOSArrAsgn enclIts line v e1 e2 :
+      let subprogram := CArrAsgn line v e1 e2 in
+      IsSubprogram program subprogram ->
+      ReachSOS (time_before subprogram enclIts) ->
+      ReachSOS (time_after subprogram enclIts)
+  | ReachSOSIfTrueB enclIts line cond c1 c2 :
+      let subprogram := CIf line cond c1 c2 in
+      IsSubprogram program subprogram ->
+      ReachSOS (time_before subprogram enclIts) ->
+      beval (time_before subprogram enclIts) cond = true ->
+      ReachSOS (time_before c1 enclIts)
+  | ReachSOSIfTrueA enclIts line cond c1 c2 :
+      let subprogram := CIf line cond c1 c2 in
+      IsSubprogram program subprogram ->
+      ReachSOS (time_after c1 enclIts) ->
+      ReachSOS (time_after subprogram enclIts)
+  | ReachSOSIfFalseB enclIts line cond c1 c2 :
+      let subprogram := CIf line cond c1 c2 in
+      IsSubprogram program subprogram ->
+      ReachSOS (time_before subprogram enclIts) ->
+      beval (time_before subprogram enclIts) cond = false ->
+      ReachSOS (time_before c2 enclIts)
+  | ReachSOSIfFalseA enclIts line cond c1 c2 :
+      let subprogram := CIf line cond c1 c2 in
+      IsSubprogram program subprogram ->
+      ReachSOS (time_after c2 enclIts) ->
+      ReachSOS (time_after subprogram enclIts)
+  | ReachSOSWhileStart enclIts line cond c :
+      let subprogram := CWhile line cond c in
+      IsSubprogram program subprogram ->
+      ReachSOS (time_before subprogram enclIts) ->
+      ReachSOS (TimepointAt (line_before subprogram + 1) (0 :: enclIts))
+  | ReachSOSWhileTrue enclIts line it cond c :
+      let subprogram := CWhile line cond c in
+      IsSubprogram program subprogram ->
+      let tBeforeIteration := TimepointAt (line_before subprogram + 1) (it :: enclIts) in
+      ReachSOS tBeforeIteration ->
+      beval tBeforeIteration cond = true ->
+      ReachSOS (time_before c (it :: enclIts))
+  | ReachSOSWhileLoop enclIts line it cond c :
+      let subprogram := CWhile line cond c in
+      IsSubprogram program subprogram ->
+      ReachSOS (time_after c (it :: enclIts)) ->
+      ReachSOS (TimepointAt (line_before subprogram + 1) (S it :: enclIts))
+  | ReachSOSWhileFalse enclIts line it cond c :
+      let subprogram := CWhile line cond c in
+      IsSubprogram program subprogram ->
+      let tBeforeIteration := TimepointAt (line_before subprogram + 1) (it :: enclIts) in
+      ReachSOS tBeforeIteration ->
+      beval tBeforeIteration cond = false ->
+      ReachSOS (time_after subprogram enclIts)
+  .
+(* NOTE: 'B' = 'before', 'A' = 'after' *)
+
+(* every rule concludes a Reach and has another conclusion alongside it *)
+Axiom SOSConclusionSkip : forall enclIts line,
+  let subprogram := CSkip line in
+  IsSubprogram program subprogram ->
+  ReachSOS (time_before subprogram enclIts) ->
+  EqAll (time_before subprogram enclIts) (time_after subprogram enclIts).
+Axiom SOSConclusionAsgn : forall enclIts line v e,
+  let subprogram := CAsgn line v e in
+  IsSubprogram program subprogram ->
+  ReachSOS (time_before subprogram enclIts) ->
+  Update (IntVarByName v) e (time_before subprogram enclIts) (time_after subprogram enclIts).
+Axiom SOSConclusionArrAsgn : forall enclIts line v e1 e2,
+  let subprogram := CArrAsgn line v e1 e2 in
+  IsSubprogram program subprogram ->
+  ReachSOS (time_before subprogram enclIts) ->
+  UpdateArray (ArrayVarByName v) e1 e2 (time_before subprogram enclIts) (time_after subprogram enclIts).
+Axiom SOSConclusionIfTrueB : forall enclIts line cond c1 c2,
+  let subprogram := CIf line cond c1 c2 in
+  IsSubprogram program subprogram ->
+  ReachSOS (time_before subprogram enclIts) ->
+  beval (time_before subprogram enclIts) cond = true ->
+  EqAll (time_before subprogram enclIts) (time_before c1 enclIts).
+Axiom SOSConclusionIfTrueA : forall enclIts line cond c1 c2,
+  let subprogram := CIf line cond c1 c2 in
+  IsSubprogram program subprogram ->
+  ReachSOS (time_after c1 enclIts) ->
+  EqAll (time_after c1 enclIts) (time_after subprogram enclIts).
+Axiom SOSConclusionIfFalseB : forall enclIts line cond c1 c2,
+  let subprogram := CIf line cond c1 c2 in
+  IsSubprogram program subprogram ->
+  ReachSOS (time_before subprogram enclIts) ->
+  beval (time_before subprogram enclIts) cond = false ->
+  EqAll (time_before subprogram enclIts) (time_before c2 enclIts).
+Axiom SOSConclusionIfFalseA : forall enclIts line cond c1 c2,
+  let subprogram := CIf line cond c1 c2 in
+  IsSubprogram program subprogram ->
+  ReachSOS (time_after c2 enclIts) ->
+  EqAll (time_after c2 enclIts) (time_after subprogram enclIts).
+Axiom SOSConclusionWhileStart : forall enclIts line cond c,
+  let subprogram := CWhile line cond c in
+  IsSubprogram program subprogram ->
+  ReachSOS (time_before subprogram enclIts) ->
+  EqAll (time_before subprogram enclIts) (TimepointAt (line_before subprogram + 1) (0 :: enclIts)).
+Axiom SOSConclusionWhileTrue : forall enclIts line cond c it,
+  let subprogram := CWhile line cond c in
+  IsSubprogram program subprogram ->
+  let tBeforeIteration := TimepointAt (line_before subprogram + 1) (it :: enclIts) in
+  ReachSOS tBeforeIteration ->
+  beval tBeforeIteration cond = true ->
+  EqAll tBeforeIteration (time_before c (it :: enclIts)).
+Axiom SOSConclusionWhileLoop : forall enclIts line it cond c,
+  let subprogram := CWhile line cond c in
+  IsSubprogram program subprogram ->
+  ReachSOS (time_after c (it :: enclIts)) ->
+  EqAll (time_after c (it :: enclIts)) (TimepointAt (line_before subprogram + 1) (S it :: enclIts)).
+Axiom SOSConclusionWhileFalse : forall enclIts line cond c it,
+  let subprogram := CWhile line cond c in
+  IsSubprogram program subprogram ->
+  let tBeforeIteration := TimepointAt (line_before subprogram + 1) (it :: enclIts) in
+  ReachSOS tBeforeIteration ->
+  beval tBeforeIteration cond = false ->
+  EqAll tBeforeIteration (time_after subprogram enclIts).
+
+
+(* Proof of W-soundness with respect to small-step operational semantics (Theorem 1) *)
+
+(* first a few lemmas *)
+
+Lemma consistent_lines_for_immediate_subprogram :
+  forall line program subprogram,
+  HasConsistentLineNumbers line program ->
+  IsImmediateSubprogram program subprogram ->
+  exists line', HasConsistentLineNumbers line' subprogram.
+Proof.
+  intros line program subprogram Hline Hsub.
+  inversion Hsub; subst;
+  inversion Hline; subst;
+  eauto.
+Qed.
+
+Lemma consistent_lines_for_subprogram :
+  forall line program,
+  HasConsistentLineNumbers line program ->
+  forall subprogram,
+  IsSubprogram program subprogram ->
+  exists line', HasConsistentLineNumbers line' subprogram.
+Proof.
+  intros line program subprogram Hline Hsub.
+  generalize dependent line.
+  induction Hsub;
+  intros line Hline.
+  - (* step *)
+    eauto using consistent_lines_for_immediate_subprogram.
+  - (* reflexive *)
+    exists line.
+    auto.
+  - (* transitive *)
+    apply IHHsub1 in Hline.
+    destruct Hline as [line' Hline'].
+    eauto.
+Qed.
+
+Definition consistent_lines_for_subprogram_of_program :=
+  consistent_lines_for_subprogram _ _ consistent_program_line_numbers.
+
+Lemma consistent_lines_implies_line_before :
+  forall line program,
+  HasConsistentLineNumbers line program ->
+  line_before program = line.
+Proof.
+  intros line program Hline.
+  inversion Hline; subst; auto.
+Qed.
+
+Lemma is_immediate_subprogram_bounds_lines :
+  forall line program,
+  HasConsistentLineNumbers line program ->
+  forall subprogram,
+  IsImmediateSubprogram program subprogram ->
+  line_before program <= line_before subprogram /\
+  line_after subprogram <= line_after program.
+Proof.
+  intros line program Hline.
+  intros subprogram Hsub.
+  inversion Hsub; subst;
+  inversion Hline; subst;
+  rename line0 into line;
+  repeat match goal with
+  | H : HasConsistentLineNumbers _ _ |- _ =>
+    apply consistent_lines_implies_line_before in H
+  end;
+  unfold line_after;
+  simpl;
+  lia.
+Qed.
+
+Lemma is_subprogram_bounds_lines :
+  forall line program,
+  HasConsistentLineNumbers line program ->
+  forall subprogram,
+  IsSubprogram program subprogram ->
+  line_before program <= line_before subprogram /\
+  line_after subprogram <= line_after program.
+Proof.
+  intros line program subprogram Hline Hsub.
+  generalize dependent line.
+  induction Hsub;
+  intros line Hline.
+  - (* step *)
+    eauto using is_immediate_subprogram_bounds_lines.
+  - (* reflexive *)
+    lia.
+  - (* transitive *)
+    eapply consistent_lines_for_subprogram in Hsub1; eauto.
+    destruct Hsub1 as [line' Hsub1].
+    apply IHHsub1 in Hline.
+    apply IHHsub2 in Hsub1.
+    lia.
+Qed.
+
+Definition is_subprogram_bounds_lines_of_program :=
+  is_subprogram_bounds_lines _ _ consistent_program_line_numbers.
+
+Lemma is_subprogram_1n :
+  forall program subprogram,
+  IsSubprogram program subprogram
+  <->
+  clos_refl_trans_1n com IsImmediateSubprogram program subprogram.
+Proof.
+  intros program subprogram.
+  split; intros Hsub;
+  induction Hsub;
+  eauto using rt1n_refl, rt1n_trans, rt_step, rt_refl, rt_trans.
+  clear Hsub1 Hsub2.
+  induction IHHsub1;
+  eauto using rt1n_trans.
+Qed.
+
+Lemma is_subprogram_next_step :
+  forall p p',
+  IsSubprogram p p' ->
+  p = p' \/
+  exists p'',
+  IsImmediateSubprogram p p'' /\
+  IsSubprogram p'' p'.
+Proof.
+  intros p p' Hsub.
+  apply is_subprogram_1n in Hsub.
+  inversion Hsub; subst; auto.
+  right.
+  exists y.
+  split; auto.
+  apply is_subprogram_1n.
+  auto.
+Qed.
+
+Lemma line_diff_non_zero :
+  forall program,
+  subprogram_line_diff program >= 1.
+Proof.
+  intros program.
+  induction program;
+  simpl;
+  lia.
+Qed.
+
+Lemma immediate_subprogram_increases_line_diff :
+  forall program subprogram,
+  IsImmediateSubprogram program subprogram ->
+  subprogram_line_diff program > subprogram_line_diff subprogram.
+Proof.
+  intros program subprogram Hsub.
+  inversion Hsub;
+  simpl; try lia.
+  - pose proof (line_diff_non_zero c2).
+    simpl; lia.
+  - pose proof (line_diff_non_zero c1).
+    simpl; lia.
+Qed.
+
+Lemma subprograms_cannot_overlap :
+  forall line p,
+  HasConsistentLineNumbers line p ->
+  forall p1 p2,
+  IsSubprogram p p1 ->
+  IsSubprogram p p2 ->
+  (
+    line_after p1 <= line_before p2
+    \/
+    line_after p2 <= line_before p1
+    \/
+    IsSubprogram p1 p2
+    \/
+    IsSubprogram p2 p1
+  ).
+Proof.
+  intros line p Hline.
+  intros p1 p2 Hsub1 Hsub2.
+  apply is_subprogram_1n in Hsub1.
+  generalize dependent line.
+  induction Hsub1 as [| p p1' p1 Himm1]; auto.
+  intros line Hline.
+  destruct (is_subprogram_next_step _ _ Hsub2) as [Heq | [p2' [Himm2 Hsub2']]].
+  - subst.
+    right. right. right.
+    apply is_subprogram_1n.
+    eauto using rt1n_trans.
+  - apply is_subprogram_1n in Hsub1.
+    destruct (consistent_lines_for_immediate_subprogram _ _ _ Hline Himm1) as [line1 Hline1].
+    specialize IHHsub1 with (line := line1) (Hline := Hline1).
+    pose proof (is_subprogram_bounds_lines _ _ Hline1 _ Hsub1) as Hbound1.
+    clear line1 Hline1.
+    destruct (consistent_lines_for_immediate_subprogram _ _ _ Hline Himm2) as [line2 Hline2].
+    pose proof (is_subprogram_bounds_lines _ _ Hline2 _ Hsub2') as Hbound2.
+    clear line2 Hline2.
+    destruct p;
+    inversion Himm1; subst;
+    inversion Himm2; subst;
+    auto;
+    clear IHHsub1;
+    inversion Hline; subst;
+    repeat match goal with
+    | H : HasConsistentLineNumbers _ _
+    |- _ =>
+      apply consistent_lines_implies_line_before in H
+    end;
+    unfold line_after in *; lia.
+Qed.
+
+Definition subprograms_of_program_cannot_overlap :=
+  subprograms_cannot_overlap _ _ consistent_program_line_numbers.
+
+
+(* we need tactics to disprove overlapping statements *)
+
+Ltac prove_impossible_overlap p1 p2 :=
+  match goal with
+  | Hsub1 : IsSubprogram program p1,
+    Hsub2 : IsSubprogram program p2
+  |- _ =>
+    let Hline1 := fresh in
+    let line1 := fresh in
+    let Hline2 := fresh in
+    let line2 := fresh in
+    (* get consistent-lines hypotheses for all subprograms of the subprograms *)
+    try match goal with | p := _ : com |- _ => constr_eq p p1; (* only do this if p1 has a local definitions *)
+      destruct (consistent_lines_for_subprogram_of_program _ Hsub1) as [line1 Hline1];
+      inversion Hline1; subst; clear Hline1
+    end;
+    destruct (consistent_lines_for_subprogram_of_program _ Hsub2) as [line2 Hline2];
+    inversion Hline2; subst; clear Hline2;
+    (* convert them to equations about line numbers *)
+    repeat match goal with
+    | H : HasConsistentLineNumbers _ _
+    |- _ =>
+      apply consistent_lines_implies_line_before in H
+    end;
+    (* get the consistent-lines hypotheses again since we lost them *)
+    destruct (consistent_lines_for_subprogram_of_program _ Hsub1) as [line1 Hline1];
+    try match goal with | p := _ : com |- _ => constr_eq p p1; (* only do this if p1 has a local definitions *)
+      inversion Hline1; subst; clear Hline1
+    end;
+    destruct (consistent_lines_for_subprogram_of_program _ Hsub2) as [line2 Hline2];
+    inversion Hline2; subst; clear Hline2;
+    (* now prove the subprograms cannot overlap *)
+    let H := fresh in
+    destruct (subprograms_of_program_cannot_overlap _ _ Hsub1 Hsub2) as [H | [H | [H | H]]];
+    unfold line_after in *; simpl in *; try lia;
+    let Heq := fresh in
+    let p := fresh in
+    let Himm := fresh in
+    let Hsub := fresh in
+    (
+      destruct (is_subprogram_next_step _ _ H) as [Heq | [p [Himm Hsub]]];
+      [
+        auto; inversion Heq; subst; simpl in *; try lia
+        |
+        (* first check if program can even contain subprograms *)
+        pose proof (line_diff_non_zero p);
+        pose proof (immediate_subprogram_increases_line_diff _ _ Himm);
+        try lia;
+        (* then compare with line bounds of every immediate subprogram *)
+        inversion Himm; subst;
+        eapply is_subprogram_bounds_lines in Hsub; eauto;
+        unfold line_after in Hsub; simpl in Hsub; try lia
+      ]
+    )
+  end.
+
+Ltac solve_impossible_overlap :=
+  try solve [
+    match goal with
+    | p1 := _ : com, p2 := _ : com
+    |- _ =>
+      prove_impossible_overlap p1 p2
+    end
+  ].
+
+
+(* lemmas about inverting reach, using the tactic *)
+
+Lemma reach_line_end_implies_line_start :
+  forall subprogramLine,
+  IsSubprogram program subprogramLine ->
+  subprogram_line_diff subprogramLine = 1 ->
+  forall enclIts,
+  ReachSOS (time_after subprogramLine enclIts) ->
+  ReachSOS (time_before subprogramLine enclIts).
+Proof.
+  intros subprogramLine HsubLine Hdiff.
+  intros enclIts Hafter.
+  inversion Hafter; subst;
+  try solve [
+    unfold line_after in H;
+    rewrite Hdiff in H;
+    simpl in H;
+    simpl in H2;
+    assert (line = line_before subprogramLine) by lia;
+    subst;
+    auto
+  ];
+  try solve [ prove_impossible_overlap subprogramLine subprogram ].
+  apply is_subprogram_bounds_lines_of_program in HsubLine.
+  unfold line_after in *.
+  lia.
+Qed.
+
+Lemma reach_seq1_start_implies_seq_start :
+  forall line c1 c2,
+  let subprogram := CSeq line c1 c2 in
+  IsSubprogram program subprogram ->
+  forall enclIts,
+  ReachSOS (time_before c1 enclIts) ->
+  ReachSOS (time_before subprogram enclIts).
+Proof.
+  intros line c1 c2 subprogram Hsub.
+  intros enclIts Hbefore.
+  unfold time_before.
+  simpl.
+  destruct (consistent_lines_for_subprogram_of_program _ Hsub) as [line' Hline].
+  inversion Hline; subst.
+  apply consistent_lines_implies_line_before in H2.
+  rewrite <- H2.
+  auto.
+Qed.
+
+Lemma reach_seq2_start_implies_seq1_end :
+  forall line c1 c2,
+  let subprogram := CSeq line c1 c2 in
+  IsSubprogram program subprogram ->
+  forall enclIts,
+  ReachSOS (time_before c2 enclIts) ->
+  ReachSOS (time_after c1 enclIts).
+Proof.
+  intros line c1 c2 subprogram Hsub.
+  intros enclIts Hbefore.
+  destruct (consistent_lines_for_subprogram_of_program _ Hsub) as [line' Hline].
+  inversion Hline; subst.
+  apply consistent_lines_implies_line_before in H2.
+  apply consistent_lines_implies_line_before in H4.
+  assert (Hmid : time_after c1 enclIts = time_before c2 enclIts). {
+    unfold time_before.
+    unfold time_after.
+    unfold line_after.
+    f_equal.
+    lia.
+  }
+  rewrite Hmid.
+  auto.
+Qed.
+
+Lemma reach_seq_end_implies_seq2_end :
+  forall line c1 c2,
+  let subprogram := CSeq line c1 c2 in
+  IsSubprogram program subprogram ->
+  forall enclIts,
+  ReachSOS (time_after subprogram enclIts) ->
+  ReachSOS (time_after c2 enclIts).
+Proof.
+  intros line c1 c2 subprogram Hsub.
+  intros enclIts Hafter.
+  destruct (consistent_lines_for_subprogram_of_program _ Hsub) as [line' Hline].
+  inversion Hline; subst.
+  apply consistent_lines_implies_line_before in H4.
+  assert (Hend : time_after c2 enclIts = time_after subprogram enclIts). {
+    unfold time_after.
+    unfold line_after.
+    f_equal.
+    simpl.
+    lia.
+  }
+  rewrite Hend.
+  auto.
+Qed.
+
+Lemma reach_if_then_start_implies_condition_true :
+  forall line cond c1 c2,
+  let subprogram := CIf line cond c1 c2 in
+  IsSubprogram program subprogram ->
+  forall enclIts,
+  ReachSOS (time_before c1 enclIts) ->
+  ReachSOS (time_before subprogram enclIts) /\
+  beval (time_before subprogram enclIts) cond = true.
+Proof.
+  intros line cond c1 c2 subprogram Hsub.
+  intros enclIts Hbefore.
+  inversion Hbefore; subst;
+  solve_impossible_overlap.
+  - destruct (consistent_lines_for_subprogram_of_program _ Hsub) as [line' Hline'].
+    inversion Hline'; subst.
+    apply consistent_lines_implies_line_before in H3.
+    apply is_subprogram_bounds_lines_of_program in Hsub.
+    cbn in *; lia.
+  - assert (Heq : subprogram = subprogram0) by solve_impossible_overlap.
+    inversion Heq; subst.
+    auto.
+Qed.
+
+Lemma reach_if_else_start_implies_condition_false :
+  forall line cond c1 c2,
+  let subprogram := CIf line cond c1 c2 in
+  IsSubprogram program subprogram ->
+  forall enclIts,
+  ReachSOS (time_before c2 enclIts) ->
+  ReachSOS (time_before subprogram enclIts) /\
+  beval (time_before subprogram enclIts) cond = false.
+Proof.
+  intros line cond c1 c2 subprogram Hsub.
+  intros enclIts Hbefore.
+  inversion Hbefore; subst;
+  solve_impossible_overlap.
+  - destruct (consistent_lines_for_subprogram_of_program _ Hsub) as [line' Hline'].
+    inversion Hline'; subst.
+    apply consistent_lines_implies_line_before in H6.
+    apply is_subprogram_bounds_lines_of_program in Hsub.
+    cbn in *; lia.
+  - assert (Heq : subprogram = subprogram0) by solve_impossible_overlap.
+    inversion Heq; subst.
+    auto.
+Qed.
+
+Lemma reach_if_end_implies_after_c1_or_c2 :
+  forall line cond c1 c2,
+  let subprogram := CIf line cond c1 c2 in
+  IsSubprogram program subprogram ->
+  forall enclIts,
+  ReachSOS (time_after subprogram enclIts) ->
+  ReachSOS (time_after c1 enclIts) \/
+  ReachSOS (time_after c2 enclIts).
+Proof.
+  intros line cond c1 c2 subprogram Hsub.
+  intros enclIts Hafter.
+  inversion Hafter; subst;
+  solve_impossible_overlap.
+  - apply is_subprogram_bounds_lines_of_program in Hsub.
+    cbn in *; lia.
+  - left.
+    assert (Heq : subprogram = subprogram0) by solve_impossible_overlap.
+    inversion Heq; subst.
+    auto.
+  - right.
+    assert (Heq : subprogram = subprogram0) by solve_impossible_overlap.
+    inversion Heq; subst.
+    auto.
+Qed.
+
+Lemma reach_first_while_condition_implies_while_start :
+  forall line cond c,
+  let subprogram := CWhile line cond c in
+  IsSubprogram program subprogram ->
+  forall enclIts,
+  ReachSOS (TimepointAt (line_before subprogram + 1) (0 :: enclIts)) ->
+  ReachSOS (time_before subprogram enclIts).
+Proof.
+  intros line cond c subprogram Hsub.
+  intros enclIts Hbefore.
+  inversion Hbefore; subst;
+  solve_impossible_overlap.
+  assert (Heq : subprogram = subprogram0) by solve_impossible_overlap.
+  inversion Heq; subst.
+  auto.
+Qed.
+
+Lemma reach_while_body_start_implies_condition_true :
+  forall line cond c,
+  let subprogram := CWhile line cond c in
+  IsSubprogram program subprogram ->
+  forall it enclIts,
+  ReachSOS (time_before c (it :: enclIts)) ->
+  let tBeforeIteration := TimepointAt (line_before subprogram + 1) (it :: enclIts) in
+  ReachSOS tBeforeIteration /\
+  beval tBeforeIteration cond = true.
+Proof.
+  intros line cond c subprogram Hsub.
+  intros it enclIts Hbefore tBeforeIteration.
+  inversion Hbefore; subst;
+  solve_impossible_overlap.
+  assert (Heq : subprogram = subprogram0) by solve_impossible_overlap.
+  inversion Heq; subst.
+  auto.
+Qed.
+
+Lemma reach_while_condition_implies_while_body_end :
+  forall line cond c,
+  let subprogram := CWhile line cond c in
+  IsSubprogram program subprogram ->
+  forall it enclIts,
+  ReachSOS (TimepointAt (line_before subprogram + 1) (S it :: enclIts)) ->
+  ReachSOS (time_after c (it :: enclIts)).
+Proof.
+  intros line cond c subprogram Hsub.
+  intros it enclIts Hbefore.
+  inversion Hbefore; subst;
+  solve_impossible_overlap.
+  assert (Heq : subprogram = subprogram0) by solve_impossible_overlap.
+  inversion Heq; subst.
+  auto.
+Qed.
+
+Lemma reach_while_end_implies_condition_false :
+  forall line cond c,
+  let subprogram := CWhile line cond c in
+  IsSubprogram program subprogram ->
+  forall enclIts,
+  ReachSOS (time_after subprogram enclIts) ->
+  exists it,
+  let tBeforeIteration := TimepointAt (line_before subprogram + 1) (it :: enclIts) in
+  ReachSOS tBeforeIteration /\
+  beval tBeforeIteration cond = false.
+Proof.
+  intros line cond c subprogram Hsub.
+  intros enclIts Hafter.
+  inversion Hafter; subst;
+  solve_impossible_overlap.
+  - apply is_subprogram_bounds_lines_of_program in Hsub.
+    cbn in *; lia.
+  - assert (Heq : subprogram = subprogram0) by solve_impossible_overlap.
+    inversion Heq; subst.
+    exists it.
+    auto.
+Qed.
+
+Lemma reach_after_implies_before :
+  forall subprogram,
+  IsSubprogram program subprogram ->
+  forall enclIts,
+  ReachSOS (time_after subprogram enclIts) ->
+  ReachSOS (time_before subprogram enclIts).
+Proof.
+  intros subprogram.
+  induction subprogram;
+  intros Hsub enclIts Hafter;
+  auto using reach_line_end_implies_line_start.
+  - (* seq *)
+    eauto 20 using
+      reach_seq1_start_implies_seq_start,
+      reach_seq2_start_implies_seq1_end,
+      reach_seq_end_implies_seq2_end,
+      IsImmediateSubprogramSeq1,
+      IsImmediateSubprogramSeq2,
+      rt_trans,
+      rt_step.
+  - (* if *)
+    destruct (reach_if_end_implies_after_c1_or_c2 _ _ _ _ Hsub _ Hafter) as [HafterThen | HafterElse].
+    + (* if then *)
+      assert (Hsub1 : IsSubprogram program subprogram1) by eauto using
+        IsImmediateSubprogramIfThen, rt_trans, rt_step.
+      assert (Hbefore1 : ReachSOS (time_before subprogram1 enclIts)) by auto.
+      destruct (reach_if_then_start_implies_condition_true _ _ _ _ Hsub _ Hbefore1) as [Hbefore _].
+      auto.
+    + (* if else *)
+      assert (Hsub2 : IsSubprogram program subprogram2) by eauto using
+        IsImmediateSubprogramIfElse, rt_trans, rt_step.
+      assert (Hbefore2 : ReachSOS (time_before subprogram2 enclIts)) by auto.
+      destruct (reach_if_else_start_implies_condition_false _ _ _ _ Hsub _ Hbefore2) as [Hbefore _].
+      auto.
+  - (* while *)
+    destruct (reach_while_end_implies_condition_false _ _ _ Hsub _ Hafter) as [it [Hbefore _]].
+    induction it.
+    + auto using reach_first_while_condition_implies_while_start.
+    + apply IHit.
+      apply reach_while_body_start_implies_condition_true;
+      eauto 20 using
+        reach_while_condition_implies_while_body_end,
+        IsImmediateSubprogramWhile,
+        rt_trans,
+        rt_step.
+Qed.
+
+Lemma while_reach_semantics :
+  forall line cond c,
+  let subprogram := CWhile line cond c in
+  IsSubprogram program subprogram ->
+  forall enclIts,
+  ReachSOS (time_after subprogram enclIts) ->
+  exists itEnd,
+  let time_before_condition := TimepointAt (line_before subprogram + 1) in
+  ReachSOS (time_before_condition (itEnd :: enclIts)) /\
+  beval (time_before_condition (itEnd :: enclIts)) cond = false /\
+  forall it,
+  it < itEnd ->
+  ReachSOS (time_before_condition (it :: enclIts)) /\
+  beval (time_before_condition (it :: enclIts)) cond = true /\
+  ReachSOS (time_after c (it :: enclIts)).
+Proof.
+  intros line cond c subprogram Hsub.
+  intros enclIts Hafter.
+  apply reach_while_end_implies_condition_false in Hafter; auto.
+  destruct Hafter as [itEnd [HbeforeCond Hcond]].
+  exists itEnd.
+  intros time_before_condition.
+  split; [| split]; auto.
+  clear Hcond.
+  induction itEnd;
+  intros it Hit;
+  inversion Hit;
+  pose proof HbeforeCond as HafterBody;
+  apply reach_while_condition_implies_while_body_end in HafterBody; auto;
+  pose proof HafterBody as HbeforeBody;
+  apply reach_after_implies_before in HbeforeBody; eauto using IsImmediateSubprogramWhile, rt_trans, rt_step;
+  pose proof HbeforeBody as Hcond';
+  eapply reach_while_body_start_implies_condition_true in Hcond'; eauto;
+  destruct Hcond' as [HbeforeCond' Hcond'];
+  auto.
+Qed.
+
+Lemma while_reach_semantics_for_last_loop_iteration :
+  forall line cond c,
+  let subprogram := CWhile line cond c in
+  IsSubprogram program subprogram ->
+  forall enclIts,
+  ReachSOS (time_after subprogram enclIts) ->
+  let itEnd := LastLoopIteration (time_before subprogram enclIts) in
+  let time_before_condition := TimepointAt (line_before subprogram + 1) in
+  ReachSOS (time_before_condition (itEnd :: enclIts)) /\
+  forall it,
+  it < itEnd ->
+  ReachSOS (time_before_condition (it :: enclIts)) /\
+  ReachSOS (time_after c (it :: enclIts)).
+Proof.
+  intros line cond c subprogram Hsub.
+  intros enclIts Hafter.
+  intros itEnd.
+  pose proof (while_reach_semantics _ _ _ Hsub _ Hafter) as Hwhile.
+  fold subprogram in Hwhile.
+  destruct Hwhile as [itEnd' [HbeforeLastCond [Hfalse Hwhile]]].
+  assert (HitEnd : itEnd = itEnd'). {
+    destruct (Nat.compare_spec itEnd itEnd') as [HitEnd | HitEnd | HitEnd]; auto.
+    - destruct (Hwhile itEnd HitEnd) as [_ [Htrue _]].
+      unfold itEnd in Htrue.
+      unfold subprogram in Htrue.
+      rewrite (last_loop_iteration_cond_is_false _ _ _ Hsub enclIts) in Htrue.
+      discriminate.
+    - unfold subprogram in Hfalse.
+      rewrite (last_loop_iteration_before_cond_is_true _ _ _ Hsub _ enclIts HitEnd) in Hfalse.
+      discriminate.
+  }
+  subst.
+  split; auto.
+  intros it Hit.
+  destruct (Hwhile it Hit) as [HbeforeCond [Htrue HafterBody]].
+  auto.
+Qed.
+
+
+(* W-soundness for subprograms *)
+Lemma trace_logic_semantics_soundness_for_subprograms :
+  forall subprogram enclIts,
+  IsSubprogram program subprogram ->
+  ReachSOS (time_after subprogram enclIts) ->
+  trace_logic_semantics enclIts subprogram.
+Proof.
+  intros subprogram.
+  induction subprogram;
+  intros enclIts Hsub Hafter;
+  assert (Hbefore : ReachSOS (time_before _ enclIts)) by eauto using reach_after_implies_before;
+  unfold trace_logic_semantics;
+  fold trace_logic_semantics.
+  - (* skip *)
+    auto using SOSConclusionSkip.
+  - (* v := e *)
+    auto using SOSConclusionAsgn.
+  - (* v:[e1] := e2 *)
+    auto using SOSConclusionArrAsgn.
+  - (* c1; c2 *)
+    eauto 20 using
+      reach_seq2_start_implies_seq1_end,
+      reach_seq_end_implies_seq2_end,
+      reach_after_implies_before,
+      IsImmediateSubprogramSeq1,
+      IsImmediateSubprogramSeq2,
+      rt_trans,
+      rt_step.
+  - (* if (cond) { c1 } else { c2 } *)
+    destruct (reach_if_end_implies_after_c1_or_c2 _ _ _ _ Hsub _ Hafter) as [HafterThen | HafterElse].
+    + assert (Hsub1 : IsSubprogram program subprogram1) by eauto using
+        IsImmediateSubprogramIfThen, rt_trans, rt_step.
+      destruct (
+        reach_if_then_start_implies_condition_true _ _ _ _ Hsub _ (
+          reach_after_implies_before _ Hsub1 _ HafterThen
+        )
+      ) as [_ Hcond].
+      rewrite Hcond.
+      eauto 10 using
+        SOSConclusionIfTrueB,
+        SOSConclusionIfTrueA,
+        reach_after_implies_before,
+        reach_if_then_start_implies_condition_true.
+    + assert (Hsub2 : IsSubprogram program subprogram2) by eauto using
+        IsImmediateSubprogramIfElse, rt_trans, rt_step.
+      destruct (
+        reach_if_else_start_implies_condition_false _ _ _ _ Hsub _ (
+          reach_after_implies_before _ Hsub2 _ HafterElse
+        )
+      ) as [_ Hcond].
+      rewrite Hcond.
+      eauto 10 using
+        SOSConclusionIfFalseB,
+        SOSConclusionIfFalseA,
+        reach_after_implies_before,
+        reach_if_else_start_implies_condition_false.
+  - (* while (cond) { c } *)
+    destruct (while_reach_semantics_for_last_loop_iteration _ _ _ Hsub _ Hafter) as [HbeforeLastCond Hwhile].
+    split; [| split; [| split]]; eauto using
+      SOSConclusionWhileStart,
+      SOSConclusionWhileFalse,
+      last_loop_iteration_cond_is_false.
+    intros it Hit.
+    destruct (Hwhile it Hit) as [HbeforeCond HafterBody].
+    split; [| split; [| split]]; eauto using
+      SOSConclusionWhileTrue,
+      SOSConclusionWhileLoop,
+      last_loop_iteration_before_cond_is_true,
+      IsImmediateSubprogramWhile,
+      rt_trans,
+      rt_step.
+Qed.
+
+(* main result: W-soundness of the semantics of the entire program *)
+Theorem trace_logic_semantics_soundness_for_program :
+  ReachSOS (time_after program (@nil nat)) ->
+  trace_logic_semantics_for_program.
+Proof.
+  eapply trace_logic_semantics_soundness_for_subprograms.
+  apply rt_refl.
+Qed.
